Add basic programs

src/set.dfy
@@ -1,6 +1,22 @@
 // TestSet1 fails to verify
-method TestSet1() returns (s: set<int>) 
-ensures s == {-4, -2, 0, 2, 4}
+// method TestSet1() {
+//   assert (set x: int | x in {-2, -1, 0, 1, 2} :: x * 2) == {-4, -2, 0, 2, 4};
+// }
+
+function Intersection<T>(s1: set<T>, s2: set<T>): set<T>
+  ensures forall x :: x in s1 && x in s2 ==> x in Intersection(s1, s2)
+  ensures forall x :: x in Intersection(s1, s2) ==> x in s1 && x in s2
 {
-  s := (set x: int | x in {-2, -1, 0, 1, 2} :: x * 2);
+  set x | x in s1 && x in s2
+}
+
+// Union fails to verify:
+// Dafny uses syntactic heuristics to determine whether a set comprehension is finite
+// The heuristics depend on type of the bound variables or conjuncts that constrain elements to be bounded
+// Dafny has no syntactic heuristic for proving a bound for disjunctions
+function Union<T>(s1: set<T>, s2: set<T>): set<T>
+  ensures forall x :: x in s1 || x in s2 ==> x in Union(s1, s2)
+  ensures forall x :: x in Union(s1, s2) ==> x in s1 || x in s2
+{
+  set x | x in s1 || x in s2
 }
