src/expt.dfy
@@ -1,0 +1,5 @@
+function expt(b: int, n: int): int
+  requires n >= 0
+{
+  if n == 0 then 1 else b * expt(b, n - 1)
+}
